theories/zoo_eio/rcfd.v
@@ -2,7 +2,8 @@ From zoo Require Import
   prelude.
 From zoo.common Require Import
   countable
-  gmultiset.
+  gmultiset
+  relations.
 From zoo.iris.base_logic Require Import
   lib.auth_gmultiset
   lib.auth_mono.
@@ -23,7 +24,7 @@ From zoo_eio Require Import
 From zoo Require Import
   options.
 
-Implicit Types b closing : bool.
+Implicit Types b owned closing : bool.
 Implicit Types ops : Z.
 Implicit Types q : Qp.
 Implicit Types qs : gmultiset Qp.
@@ -34,6 +35,7 @@ Implicit Types o : option val.
 Record metadata := {
   metadata_fd : val ;
   metadata_open : block_id ;
+  metadata_owned : bool ;
   metadata_tokens : gname ;
   metadata_lstate : gname ;
 }.
@@ -72,6 +74,16 @@ Inductive lstate :=
   | LClosingNoUsers.
 Implicit Types lstate : lstate.
 
+#[local] Definition lstate_measure lstate :=
+  match lstate with
+  | LOpen =>
+      0
+  | LClosingUsers =>
+      1
+  | LClosingNoUsers =>
+      2
+  end.
+
 #[global] Instance lstate_inhabited : Inhabited lstate :=
   populate LOpen.
 #[global] Instance lstate_eq_dec : EqDecision lstate :=
@@ -83,6 +95,36 @@ Inductive lstep : relation lstate :=
   | lstep_close_no_users :
       lstep LClosingUsers LClosingNoUsers.
 #[local] Hint Constructors lstep : core.
+
+#[local] Lemma lstep_measure lstate1 lstate2 :
+  lstep lstate1 lstate2 →
+  lstate_measure lstate1 < lstate_measure lstate2.
+Proof.
+  intros []; simpl; lia.
+Qed.
+#[local] Lemma lstep_tc_measure lstate1 lstate2 :
+  tc lstep lstate1 lstate2 →
+  lstate_measure lstate1 < lstate_measure lstate2.
+Proof.
+  intros Hlsteps.
+  apply transitive_tc; first apply _.
+  eapply (tc_congruence lstate_measure); last done.
+  apply lstep_measure.
+Qed.
+#[local] Lemma lstep_rtc_measure lstate1 lstate2 :
+  rtc lstep lstate1 lstate2 →
+  lstate_measure lstate1 ≤ lstate_measure lstate2.
+Proof.
+  intros [<- | Hlsteps%lstep_tc_measure]%rtc_tc; lia.
+Qed.
+
+#[local] Instance lsteps_antisymm :
+  AntiSymm (=) (rtc lstep).
+Proof.
+  intros lstate1 lstate2 Hlsteps1 Hlsteps2%lstep_rtc_measure.
+  apply rtc_tc in Hlsteps1 as [<- | Hlsteps1%lstep_tc_measure]; first done.
+  lia.
+Qed.
 
 Class RcfdG Σ `{zoo_G : !ZooG Σ} := {
   #[local] rcfd_G_spsc_waiter_G :: SpscWaiterG Σ ;
@@ -114,21 +156,33 @@ Section rcfd_G.
   #[local] Definition tokens_frag γ q :=
     auth_gmultiset_frag γ.(metadata_tokens) {[+q+]}.
 
-  #[local] Definition lstate_auth' γ_lstate lstate :=
-    auth_mono_auth _ γ_lstate (DfracOwn 1) lstate.
+  #[local] Definition lstate_auth_frac owned lstate :=
+    match lstate with
+    | LOpen =>
+        if owned then 1/4 else 1
+    | _ =>
+        1
+    end%Qp.
+  #[local] Definition lstate_auth' γ_lstate owned lstate :=
+    auth_mono_auth _ γ_lstate (DfracOwn $ lstate_auth_frac owned lstate) lstate.
   #[local] Definition lstate_auth γ lstate :=
-    lstate_auth' γ.(metadata_lstate) lstate.
+    lstate_auth' γ.(metadata_lstate) γ.(metadata_owned) lstate.
   #[local] Definition lstate_lb γ lstate :=
     auth_mono_lb _ γ.(metadata_lstate) lstate.
 
-  #[local] Definition inv_inner_open γ Ψ state ops : iProp Σ :=
+  #[local] Definition owner' γ_lstate :=
+    auth_mono_auth _ γ_lstate (DfracOwn (3/4)%Qp) LOpen.
+  #[local] Definition owner γ :=
+    owner' γ.(metadata_lstate).
+
+  #[local] Definition inv_lstate_open γ Ψ state ops : iProp Σ :=
     ∃ q qs,
     tokens_auth γ qs ∗
     ⌜state = Open⌝ ∗
     ⌜ops = size qs⌝ ∗
     ⌜set_fold Qp.add q qs = 1%Qp⌝ ∗
     Ψ q.
-  #[local] Instance : CustomIpatFormat "inv_inner_open" :=
+  #[local] Instance : CustomIpatFormat "inv_lstate_open" :=
     "(
       %q{} &
       %qs{} &
@@ -138,7 +192,7 @@ Section rcfd_G.
       %Hqs{} &
       HΨ{_{!}}
     )".
-  #[local] Definition inv_inner_closing_users γ Ψ state ops : iProp Σ :=
+  #[local] Definition inv_lstate_closing_users γ Ψ state ops : iProp Σ :=
     ∃ q qs fn,
     tokens_auth γ qs ∗
     ⌜state = Closing fn⌝ ∗
@@ -147,7 +201,7 @@ Section rcfd_G.
     ⌜set_fold Qp.add q qs = 1%Qp⌝ ∗
     Ψ q ∗
     (Ψ 1%Qp -∗ WP fn () {{ itype_unit }}).
-  #[local] Instance : CustomIpatFormat "inv_inner_closing_users" :=
+  #[local] Instance : CustomIpatFormat "inv_lstate_closing_users" :=
     "(
       %q{} &
       %qs{} &
@@ -160,29 +214,32 @@ Section rcfd_G.
       HΨ{_{!}} &
       Hfn{}
     )".
-  #[local] Definition inv_inner_closing_no_users state : iProp Σ :=
+  #[local] Definition inv_lstate_closing_no_users state : iProp Σ :=
     ∃ fn,
     ⌜state = Closing fn⌝ ∗
     WP fn () {{ itype_unit }}.
-  #[local] Instance : CustomIpatFormat "inv_inner_closing_no_users" :=
+  #[local] Instance : CustomIpatFormat "inv_lstate_closing_no_users" :=
     "(
       %fn{} &
       {%H{eq};->} &
       Hfn{}
     )".
+  #[local] Definition inv_lstate l γ Ψ state lstate ops :=
+    match lstate with
+    | LOpen =>
+        inv_lstate_open γ Ψ state ops
+    | LClosingUsers =>
+        inv_lstate_closing_users γ Ψ state ops
+    | LClosingNoUsers =>
+        inv_lstate_closing_no_users state
+    end.
+
   #[local] Definition inv_inner l γ Ψ : iProp Σ :=
     ∃ state lstate ops,
     l.[ops] ↦ #ops ∗
     l.[state] ↦ state_to_val γ state ∗
     lstate_auth γ lstate ∗
-    match lstate with
-    | LOpen =>
-        inv_inner_open γ Ψ state ops
-    | LClosingUsers =>
-        inv_inner_closing_users γ Ψ state ops
-    | LClosingNoUsers =>
-        inv_inner_closing_no_users state
-    end.
+    inv_lstate l γ Ψ state lstate ops.
   #[local] Instance : CustomIpatFormat "inv_inner" :=
     "(
       %state{} &
@@ -195,9 +252,10 @@ Section rcfd_G.
     )".
   #[local] Definition inv' l γ Ψ :=
     inv nroot (inv_inner l γ Ψ).
-  Definition rcfd_inv t fd Ψ : iProp Σ :=
+  Definition rcfd_inv t owned fd Ψ : iProp Σ :=
     ∃ l γ,
     ⌜t = #l⌝ ∗
+    ⌜owned = γ.(metadata_owned)⌝ ∗
     ⌜fd = γ.(metadata_fd)⌝ ∗
     meta l nroot γ ∗
     inv' l γ Ψ.
@@ -207,8 +265,23 @@ Section rcfd_G.
       %γ &
       -> &
       -> &
+      -> &
       #Hmeta &
       #Hinv
+    )".
+
+  Definition rcfd_owner t : iProp Σ :=
+    ∃ l γ,
+    ⌜t = #l⌝ ∗
+    meta l nroot γ ∗
+    owner γ.
+  #[local] Instance : CustomIpatFormat "owner" :=
+    "(
+      %l{;_} &
+      %γ{;_} &
+      %Heq{} &
+      #Hmeta_{} &
+      Howner{_{}}
     )".
 
   Definition rcfd_closing t : iProp Σ :=
@@ -218,39 +291,44 @@ Section rcfd_G.
     lstate_lb γ LClosingUsers.
   #[local] Instance : CustomIpatFormat "closing" :=
     "(
-      %l_ &
-      %γ_ &
-      %Heq &
-      #Hmeta_ &
-      #Hlstate_lb
+      %l{;_} &
+      %γ{;_} &
+      %Heq{} &
+      #Hmeta_{} &
+      #Hlstate_lb{_{}}
     )".
 
-  #[global] Instance rcfd_inv_contractive t fd n :
+  #[global] Instance rcfd_inv_contractive t owned fd n :
     Proper (
       (pointwise_relation _ (dist_later n)) ==>
       (≡{n}≡)
-    ) (rcfd_inv t fd).
+    ) (rcfd_inv t owned fd).
   Proof.
-    rewrite /rcfd_inv /inv' /inv_inner /inv_inner_open /inv_inner_closing_users.
+    rewrite /rcfd_inv /inv' /inv_inner /inv_lstate /inv_lstate_open /inv_lstate_closing_users.
     solve_contractive.
   Qed.
-  #[global] Instance rcfd_inv_proper t fd :
+  #[global] Instance rcfd_inv_proper t owned fd :
     Proper (
       (pointwise_relation _ (≡)) ==>
       (≡)
-    ) (rcfd_inv t fd).
+    ) (rcfd_inv t owned fd).
   Proof.
-    rewrite /rcfd_inv /inv' /inv_inner /inv_inner_open /inv_inner_closing_users.
+    rewrite /rcfd_inv /inv' /inv_inner /inv_lstate /inv_lstate_open /inv_lstate_closing_users.
     solve_proper.
   Qed.
 
+  #[global] Instance rcfd_owner_timeless t :
+    Timeless (rcfd_owner t).
+  Proof.
+    apply _.
+  Qed.
   #[global] Instance rcfd_closing_timeless t :
     Timeless (rcfd_closing t).
   Proof.
     apply _.
   Qed.
-  #[global] Instance rcfd_inv_persistent t fd Ψ :
-    Persistent (rcfd_inv t fd Ψ).
+  #[global] Instance rcfd_inv_persistent t owned fd Ψ :
+    Persistent (rcfd_inv t owned fd Ψ).
   Proof.
     apply _.
   Qed.
@@ -289,12 +367,20 @@ Section rcfd_G.
     apply auth_gmultiset_update_dealloc.
   Qed.
 
-  #[local] Lemma lstate_alloc :
+  #[local] Lemma lstate_owner_alloc owned :
     ⊢ |==>
       ∃ γ_lstate,
-      lstate_auth' γ_lstate LOpen.
+      lstate_auth' γ_lstate owned LOpen ∗
+      if owned then
+        owner' γ_lstate
+      else
+        True.
   Proof.
-    apply auth_mono_alloc.
+    iMod (auth_mono_alloc (auth_mono_G := rcfd_G_lstate_G) _ LOpen) as "(%γ_lstate & Hauth)".
+    destruct owned; last iSteps.
+    iEval (rewrite -Qp.quarter_three_quarter) in "Hauth".
+    iDestruct "Hauth" as "(Hauth & Howner)".
+    iSteps.
   Qed.
   #[local] Lemma lstate_lb_get γ lstate :
     lstate_auth γ lstate ⊢
@@ -319,43 +405,210 @@ Section rcfd_G.
   #[local] Lemma lstate_valid_closing_users γ lstate :
     lstate_auth γ lstate -∗
     lstate_lb γ LClosingUsers -∗
-    ⌜lstate = LClosingUsers ∨ lstate = LClosingNoUsers⌝.
+    ⌜lstate ≠ LOpen⌝.
   Proof.
-    iIntros "Hlstate_auth Hlstate_lb".
-    iDestruct (lstate_valid with "Hlstate_auth Hlstate_lb") as %Hlsteps.
+    iIntros "Hauth Hlb".
+    iDestruct (lstate_valid with "Hauth Hlb") as %Hlsteps.
     iPureIntro.
     apply rtc_inv in Hlsteps as [<- | (lstate' & Hlstep & Hlsteps)]; first naive_solver.
     invert Hlstep.
     apply rtc_inv in Hlsteps as [<- | (lstate' & Hlstep & Hlsteps)]; first naive_solver.
     invert Hlstep.
+  Qed.
+  #[local] Lemma lstate_valid_closing_users' γ lstate :
+    lstate_auth γ lstate -∗
+    lstate_lb γ LClosingUsers -∗
+    ⌜lstate = LClosingUsers ∨ lstate = LClosingNoUsers⌝.
+  Proof.
+    iIntros "Hauth Hlb".
+    iDestruct (lstate_valid_closing_users with "Hauth Hlb") as %Hlstate.
+    destruct lstate; iSteps.
   Qed.
   #[local] Lemma lstate_valid_closing_no_users γ lstate :
     lstate_auth γ lstate -∗
     lstate_lb γ LClosingNoUsers -∗
     ⌜lstate = LClosingNoUsers⌝.
   Proof.
-    iIntros "Hlstate_auth Hlstate_lb".
-    iDestruct (lstate_valid with "Hlstate_auth Hlstate_lb") as %Hlsteps.
+    iIntros "Hauth Hlb".
+    iDestruct (lstate_valid with "Hauth Hlb") as %Hlsteps.
     iPureIntro.
     apply rtc_inv in Hlsteps as [<- | (lstate' & Hlstep & Hlsteps)]; first naive_solver.
     invert Hlstep.
   Qed.
-  #[local] Lemma lstate_update {γ lstate} lstate' :
-    lstep lstate lstate' →
-    lstate_auth γ lstate ⊢ |==>
-    lstate_auth γ lstate'.
+  #[local] Lemma lstate_update_close_users γ :
+    lstate_auth γ LOpen -∗
+    (if γ.(metadata_owned) then owner γ else True) ==∗
+    lstate_auth γ LClosingUsers.
   Proof.
-    apply auth_mono_update'.
+    iIntros "Hauth Howner".
+    iAssert (auth_mono_auth (auth_mono_G := rcfd_G_lstate_G) _ γ.(metadata_lstate) (DfracOwn 1) LOpen) with "[Hauth Howner]" as "Hauth".
+    { rewrite /lstate_auth /lstate_auth' /=.
+      destruct γ.(metadata_owned); last iSteps.
+      iCombine "Hauth Howner" as "Hauth".
+      iEval (rewrite Qp.quarter_three_quarter) in "Hauth".
+      iSteps.
+    }
+    iApply (auth_mono_update' with "Hauth"); first done.
+  Qed.
+  #[local] Lemma lstate_update_close_no_users γ :
+    lstate_auth γ LClosingUsers ⊢ |==>
+    lstate_auth γ LClosingNoUsers.
+  Proof.
+    apply auth_mono_update'; first done.
   Qed.
 
-  Lemma rcfd_make_spec Ψ fd :
+  #[local] Lemma owner_exclusive γ :
+    owner γ -∗
+    owner γ -∗
+    False.
+  Proof.
+    iIntros "Hauth_1 Hauth_2".
+    iDestruct (auth_mono_auth_valid_2 with "Hauth_1 Hauth_2") as "(% & _)". done.
+  Qed.
+  #[local] Lemma owner_lstate_auth γ lstate :
+    owner γ -∗
+    lstate_auth γ lstate -∗
+    ⌜lstate = LOpen⌝.
+  Proof.
+    iIntros "Howner Hauth".
+    iApply (auth_mono_auth_agree_L with "Hauth Howner").
+  Qed.
+  #[local] Lemma owner_lstate_lb γ :
+    owner γ -∗
+    lstate_lb γ LClosingUsers -∗
+    False.
+  Proof.
+    iIntros "Hauth Hlb".
+    iDestruct (auth_mono_lb_valid with "Hauth Hlb") as %H%lstep_rtc_measure.
+    exfalso. simpl in H. lia.
+  Qed.
+
+  #[local] Lemma rcfd_owner_elim l γ :
+    meta l nroot γ -∗
+    rcfd_owner #l -∗
+    owner γ.
+  Proof.
+    iIntros "#Hmeta (:owner)". injection Heq as <-.
+    iDestruct (meta_agree with "Hmeta Hmeta_") as %<-.
+    iSteps.
+  Qed.
+  #[local] Lemma rcfd_owner_elim' l γ b :
+    meta l nroot γ -∗
+    ( if b then
+        rcfd_owner #l
+      else
+        True
+    ) -∗
+    if b then
+      owner γ
+    else
+      True.
+  Proof.
+    iIntros "#Hmeta Howner".
+    destruct b; last iSteps.
+    iApply (rcfd_owner_elim with "Hmeta Howner").
+  Qed.
+  Lemma rcfd_owner_exclusive t :
+    rcfd_owner t -∗
+    rcfd_owner t -∗
+    False.
+  Proof.
+    iIntros "(:owner =1) (:owner =2)". simplify.
+    iDestruct (meta_agree with "Hmeta_1 Hmeta_2") as %->.
+    iApply (owner_exclusive with "Howner_1 Howner_2").
+  Qed.
+  Lemma rcfd_owner_closing t :
+    rcfd_owner t -∗
+    rcfd_closing t -∗
+    False.
+  Proof.
+    iIntros "(:owner =1) (:closing =2)". simplify.
+    iDestruct (meta_agree with "Hmeta_1 Hmeta_2") as %->.
+    iApply (owner_lstate_lb with "Howner_1 Hlstate_lb_2").
+  Qed.
+
+  #[local] Lemma rcfd_closing_elim l γ :
+    meta l nroot γ -∗
+    rcfd_closing #l -∗
+    lstate_lb γ LClosingUsers.
+  Proof.
+    iIntros "#Hmeta (:closing)". injection Heq as <-.
+    iDestruct (meta_agree with "Hmeta Hmeta_") as %<-.
+    iSteps.
+  Qed.
+  #[local] Lemma rcfd_closing_elim' l γ b P :
+    meta l nroot γ -∗
+    ( if b then
+        rcfd_closing #l
+      else
+        P
+    ) -∗
+    if b then
+      lstate_lb γ LClosingUsers
+    else
+      P.
+  Proof.
+    iIntros "#Hmeta Hclosing".
+    destruct b; last iSteps.
+    iApply (rcfd_closing_elim with "Hmeta Hclosing").
+  Qed.
+
+  #[local] Lemma inv_lstate_Open l γ Ψ lstate ops :
+    inv_lstate l γ Ψ Open lstate ops ⊢
+    ⌜lstate = LOpen⌝.
+  Proof.
+    destruct lstate; iSteps.
+  Qed.
+  #[local] Lemma inv_lstate_Closing l γ Ψ state lstate ops :
+    state ≠ Open →
+    inv_lstate l γ Ψ state lstate ops -∗
+    lstate_auth γ lstate -∗
+      ∃ fn,
+      ⌜state = Closing fn⌝ ∗
+      ⌜lstate ≠ LOpen ⌝ ∗
+      lstate_lb γ LClosingUsers.
+  Proof.
+    iIntros "%Hlstate Hlstate Hlstate_auth".
+    iDestruct (lstate_lb_get with "Hlstate_auth") as "Hlstate_lb".
+    destruct lstate.
+    - iDestruct "Hlstate" as "(:inv_lstate_open)".
+      exfalso. done.
+    - iDestruct "Hlstate" as "(:inv_lstate_closing_users)".
+      iSteps.
+    - iDestruct "Hlstate" as "(:inv_lstate_closing_no_users)".
+      iDestruct (lstate_lb_mono with "Hlstate_lb") as "$"; first done.
+      iSteps.
+  Qed.
+  #[local] Lemma inv_lstate_LClosing l γ Ψ state lstate ops :
+    lstate ≠ LOpen →
+    inv_lstate l γ Ψ state lstate ops -∗
+    lstate_auth γ lstate -∗
+      ∃ fn,
+      ⌜state = Closing fn⌝ ∗
+      lstate_lb γ LClosingUsers.
+  Proof.
+    iIntros "%Hlstate Hlstate Hlstate_auth".
+    iDestruct (lstate_lb_get with "Hlstate_auth") as "Hlstate_lb".
+    destruct lstate; first done.
+    - iDestruct "Hlstate" as "(:inv_lstate_closing_users)".
+      iSteps.
+    - iDestruct "Hlstate" as "(:inv_lstate_closing_no_users)".
+      iDestruct (lstate_lb_mono with "Hlstate_lb") as "$"; first done.
+      iSteps.
+  Qed.
+
+  Lemma rcfd_make_spec owned Ψ fd :
     {{{
       Ψ 1%Qp
     }}}
       rcfd_make fd
     {{{ t,
       RET t;
-      rcfd_inv t fd Ψ
+      rcfd_inv t owned fd Ψ ∗
+      if owned then
+        rcfd_owner t
+      else
+        True
     }}}.
   Proof.
     iIntros "%Φ HΨ HΦ".
@@ -365,17 +618,21 @@ Section rcfd_G.
     wp_block l as "Hmeta" "(Hl_ops & Hl_fd & _)".
 
     iMod tokens_alloc as "(%γ_tokens & Htokens_auth)".
-    iMod lstate_alloc as "(%γ_lstate & Hlstate_auth)".
+    iMod (lstate_owner_alloc owned) as "(%γ_lstate & Hlstate_auth & Howner)".
+
     pose γ := {|
       metadata_fd := fd ;
       metadata_open := open ;
+      metadata_owned := owned ;
       metadata_tokens := γ_tokens ;
       metadata_lstate := γ_lstate ;
     |}.
     iMod (meta_set γ with "Hmeta") as "#Hmeta"; first done.
 
     iApply "HΦ".
-    iExists l, γ. iSteps. iExists Open. iSteps.
+    iSplitR "Howner".
+    - iExists l, γ. iSteps. iExists Open. iSteps.
+    - destruct owned; iSteps.
   Qed.
 
   #[local] Lemma rcfd_finish_spec l γ Ψ (close : val) :
@@ -396,13 +653,13 @@ Section rcfd_G.
     wp_bind (_.{ops})%E.
     iInv "Hinv" as "(:inv_inner =1)".
     wp_load.
-    iDestruct (lstate_valid_closing_users with "Hlstate_auth Hlstate_lb") as %[-> | ->].
+    iDestruct (lstate_valid_closing_users' with "Hlstate_auth Hlstate_lb") as %[-> | ->].
 
-    - iDestruct "Hlstate" as "(:inv_inner_closing_users =1)".
+    - iDestruct "Hlstate" as "(:inv_lstate_closing_users =1)".
       iSplitR "HΦ". { iFrameSteps 2. }
       iSteps.
 
-    - iDestruct "Hlstate" as "(:inv_inner_closing_no_users =1)".
+    - iDestruct "Hlstate" as "(:inv_lstate_closing_no_users =1)".
       iDestruct (lstate_lb_get with "Hlstate_auth") as "{Hlstate_lb} #Hlstate_lb".
       iSplitR "HΦ". { iFrameSteps 2. }
       iIntros "!> {%}".
@@ -416,7 +673,7 @@ Section rcfd_G.
       destruct state2; first zoo_simpl.
       destruct Hcas as (_ & _ & [= <-]).
       iDestruct (lstate_valid_closing_no_users with "Hlstate_auth Hlstate_lb") as %->.
-      iDestruct "Hlstate" as "(:inv_inner_closing_no_users =2 eq)". injection Heq as <-.
+      iDestruct "Hlstate" as "(:inv_lstate_closing_no_users =2 eq)". injection Heq as <-.
       iSplitR "Hfn2 HΦ".
       { iExists (Closing _). iFrameSteps. }
       iSteps.
@@ -447,10 +704,10 @@ Section rcfd_G.
     iSplitR "HΦ".
     { iDestruct "H" as "[#Hlstate_lb | (%q & Htokens_frag & HΨ)]".
       - iDestruct (lstate_valid_closing_no_users with "Hlstate_auth Hlstate_lb") as %->.
-        iDestruct "Hlstate" as "(:inv_inner_closing_no_users =1)".
+        iDestruct "Hlstate" as "(:inv_lstate_closing_no_users =1)".
         iFrameSteps 2.
       - destruct lstate1.
-        + iDestruct "Hlstate" as "(:inv_inner_open =1 !=)".
+        + iDestruct "Hlstate" as "(:inv_lstate_open =1 !=)".
           iDestruct (tokens_elem_of with "Htokens_auth Htokens_frag") as %Hq.
           iMod (tokens_update_dealloc with "Htokens_auth Htokens_frag") as "Htokens_auth".
           iDestruct (fractional with "[$HΨ $HΨ_]") as "HΨ".
@@ -459,14 +716,14 @@ Section rcfd_G.
             rewrite gmultiset_size_difference; first multiset_solver.
             rewrite gmultiset_size_singleton. lia.
           * rewrite (gmultiset_disj_union_difference' q qs1) // gmultiset_set_fold_disj_union gmultiset_set_fold_singleton // in Hqs1.
-        + iDestruct "Hlstate" as "(:inv_inner_closing_users =1 !=)".
+        + iDestruct "Hlstate" as "(:inv_lstate_closing_users =1 !=)".
           iDestruct (tokens_elem_of with "Htokens_auth Htokens_frag") as %Hq.
           destruct (decide (size qs1 = 1)) as [Hqs_size' | Hqs_size'].
           * apply gmultiset_size_1_elem_of in Hqs_size' as (q_ & ->%leibniz_equiv). rewrite gmultiset_set_fold_singleton in Hqs1.
             apply gmultiset_elem_of_singleton in Hq as <-.
             iMod (tokens_update_dealloc with "Htokens_auth Htokens_frag") as "Htokens_auth".
             rewrite gmultiset_difference_diag.
-            iMod (lstate_update LClosingNoUsers with "Hlstate_auth") as "Hlstate_auth"; first done.
+            iMod (lstate_update_close_no_users with "Hlstate_auth") as "Hlstate_auth".
             iDestruct (fractional with "[$HΨ $HΨ_]") as "HΨ". rewrite Hqs1.
             iFrameSteps 2.
           * iMod (tokens_update_dealloc with "Htokens_auth Htokens_frag") as "Htokens_auth".
@@ -477,7 +734,7 @@ Section rcfd_G.
             -- rewrite gmultiset_size_difference; first multiset_solver.
                rewrite gmultiset_size_singleton. lia.
             -- rewrite (gmultiset_disj_union_difference' q qs1) // gmultiset_set_fold_disj_union gmultiset_set_fold_singleton // in Hqs1.
-        + iDestruct "Hlstate" as "(:inv_inner_closing_no_users =1)".
+        + iDestruct "Hlstate" as "(:inv_lstate_closing_no_users =1)".
           iFrameSteps 2.
     }
     iIntros "!> {%}".
@@ -490,31 +747,159 @@ Section rcfd_G.
     wp_load.
     destruct (decide (lstate2 = LOpen)) as [-> | Hlstate2].
 
-    - iDestruct "Hlstate" as "(:inv_inner_open =2)".
+    - iDestruct "Hlstate" as "(:inv_lstate_open =2)".
       iSplitR "HΦ". { iFrameSteps 2. }
       iSteps.
 
-    - iAssert (
-        ∃ fn2,
-        ⌜state2 = Closing fn2⌝ ∗
-        lstate_lb γ LClosingUsers
-      )%I as "(%fn2 & -> & #Hlstate_lb)".
-      { destruct lstate2; first done.
-        - iDestruct "Hlstate" as "(:inv_inner_closing_users =2)".
-          iDestruct (lstate_lb_get with "Hlstate_auth") as "$".
-          iSteps.
-        - iDestruct "Hlstate" as "(:inv_inner_closing_no_users =2)".
-          iDestruct (lstate_lb_get with "Hlstate_auth") as "Hlstate_lb".
-          iDestruct (lstate_lb_mono LClosingUsers with "Hlstate_lb") as "$"; first done.
-          iSteps.
-      }
-
+    - iDestruct (inv_lstate_LClosing with "Hlstate Hlstate_auth") as "(%fn2 & -> & #Hlstate_lb)"; first done.
       iSplitR "HΦ". { iFrameSteps 2. }
       iIntros "!> {%}".
 
       wp_smart_apply (rcfd_finish_spec with "[$] HΦ").
   Qed.
 
+  Inductive specification :=
+    | SpecOwner
+    | SpecClosing
+    | SpecNormal.
+  Implicit Types spec : specification.
+
+  #[local] Instance specification_eq_dec : EqDecision specification :=
+    ltac:(solve_decision).
+
+  #[local] Definition specification_pre_1 t spec : iProp Σ :=
+    match spec with
+    | SpecOwner =>
+        rcfd_owner t
+    | SpecClosing =>
+        rcfd_closing t
+    | SpecNormal =>
+        True
+    end.
+  #[local] Definition specification_pre_2 γ spec : iProp Σ :=
+    match spec with
+    | SpecOwner =>
+        owner γ
+    | SpecClosing =>
+        lstate_lb γ LClosingUsers
+    | SpecNormal =>
+        True
+    end.
+  #[local] Lemma specification_pre_1_2 l γ spec :
+    meta l nroot γ -∗
+    specification_pre_1 #l spec -∗
+    specification_pre_2 γ spec.
+  Proof.
+    iIntros "#Hmeta Hspec".
+    destruct spec; last iSteps.
+    - iApply (rcfd_owner_elim with "Hmeta Hspec").
+    - iApply (rcfd_closing_elim with "Hmeta Hspec").
+  Qed.
+
+  #[local] Lemma rcfd_get_spec_aux spec l γ Ψ `{HΨ : !Fractional Ψ} :
+    {{{
+      inv' l γ Ψ ∗
+      specification_pre_2 γ spec
+    }}}
+      rcfd_get #l
+    {{{ o,
+      RET (o : val);
+      match spec with
+      | SpecOwner =>
+          ⌜o ≠ None⌝ ∗
+          owner γ
+      | SpecClosing =>
+          ⌜o = None⌝
+      | SpecNormal =>
+          True
+      end ∗
+      match o with
+      | None =>
+          True
+      | Some fd_ =>
+          ∃ q,
+          ⌜fd_ = γ.(metadata_fd)⌝ ∗
+          tokens_frag γ q ∗
+          Ψ q
+      end
+    }}}.
+  Proof.
+    iIntros "%Φ (#Hinv & Hspec) HΦ".
+
+    wp_rec. wp_pures.
+
+    wp_bind (FAA _ _).
+    iInv "Hinv" as "(:inv_inner =1)".
+    wp_faa.
+
+    iAssert (|==>
+      inv_inner l γ Ψ ∗
+      ( lstate_lb γ LClosingNoUsers
+      ∨ ∃ q,
+        tokens_frag γ q ∗
+        Ψ q
+      )
+    )%I with "[- Hspec HΦ]" as ">($ & H)".
+    { destruct lstate1.
+      - iDestruct "Hlstate" as "(:inv_lstate_open)".
+        iMod (tokens_update_alloc (q / 2) with "Htokens_auth") as "(Htokens_auth & Htokens_frag)".
+        iDestruct (fractional_half with "HΨ") as "(HΨ1 & HΨ2)"; first done.
+        iSplitR "Htokens_frag HΨ2"; last iSteps.
+        iFrameSteps 2; iPureIntro.
+        + rewrite gmultiset_size_disj_union gmultiset_size_singleton. lia.
+        + rewrite gmultiset_set_fold_disj_union gmultiset_set_fold_singleton Qp.div_2 //.
+      - iDestruct "Hlstate" as "(:inv_lstate_closing_users)".
+        iMod (tokens_update_alloc (q / 2) with "Htokens_auth") as "(Htokens_auth & Htokens_frag)".
+        iDestruct (fractional_half with "HΨ") as "(HΨ1 & HΨ2)"; first done.
+        iSplitR "Htokens_frag HΨ2"; last iSteps.
+        iFrameSteps 2; iPureIntro.
+        + rewrite gmultiset_size_disj_union gmultiset_size_singleton. lia.
+        + rewrite gmultiset_size_disj_union. lia.
+        + rewrite gmultiset_set_fold_disj_union gmultiset_set_fold_singleton Qp.div_2 //.
+      - iDestruct "Hlstate" as "(:inv_lstate_closing_no_users)".
+        iDestruct (lstate_lb_get with "Hlstate_auth") as "#Hlstate_lb".
+        iFrameSteps 2.
+    }
+
+    iModIntro. wp_pures. clear- HΨ.
+
+    wp_bind (_.{state})%E.
+    iInv "Hinv" as "(:inv_inner =2)".
+    wp_load.
+    destruct (decide (lstate2 = LOpen)) as [-> | Hlstate2].
+
+    - iDestruct "Hlstate" as "(:inv_lstate_open)".
+
+      iDestruct "H" as "[#Hlstate_lb | (%q' & Htokens_frag & HΨ_)]".
+      { iDestruct (lstate_valid_closing_no_users with "Hlstate_auth Hlstate_lb") as %?. done. }
+
+      iAssert ⌜spec ≠ SpecClosing⌝%I as %Hspec.
+      { iIntros (->).
+        iDestruct (lstate_valid_closing_users with "Hlstate_auth Hspec") as %?. congruence.
+      }
+
+      iSplitR "Hspec Htokens_frag HΨ_ HΦ". { iFrameSteps 2. }
+      iModIntro. clear- Hspec.
+
+      wp_pures.
+      iApply ("HΦ" $! (Some _)).
+      destruct spec; try congruence; iSteps.
+
+    - iDestruct (inv_lstate_LClosing with "Hlstate Hlstate_auth") as "#(%fn2 & -> & _)"; first done.
+
+      iAssert ⌜spec ≠ SpecOwner⌝%I as %Hspec.
+      { iIntros (->).
+        iDestruct (owner_lstate_auth with "Hspec Hlstate_auth") as %->. congruence.
+      }
+
+      iSplitR "H HΦ". { iFrameSteps 2. }
+      iModIntro. clear- HΨ Hspec.
+
+      wp_smart_apply (rcfd_put_spec with "[$]") as "_".
+      wp_pures.
+      iApply ("HΦ" $! None).
+      destruct spec; try congruence; iSteps.
+  Qed.
   #[local] Lemma rcfd_get_spec l γ Ψ `{HΨ : !Fractional Ψ} :
     {{{
       inv' l γ Ψ
@@ -535,74 +920,107 @@ Section rcfd_G.
   Proof.
     iIntros "%Φ #Hinv HΦ".
 
-    wp_rec. wp_pures.
+    wp_apply (rcfd_get_spec_aux SpecNormal with "[$]").
+    iSteps.
+  Qed.
+  #[local] Lemma rcfd_get_spec_owner l γ Ψ `{HΨ : !Fractional Ψ} :
+    {{{
+      inv' l γ Ψ ∗
+      owner γ
+    }}}
+      rcfd_get #l
+    {{{
+      RET Some γ.(metadata_fd) : val;
+      ∃ q,
+      owner γ ∗
+      tokens_frag γ q ∗
+      Ψ q
+    }}}.
+  Proof.
+    iIntros "%Φ (#Hinv & Howner) HΦ".
 
-    wp_bind (FAA _ _).
-    iInv "Hinv" as "(:inv_inner =1)".
-    wp_faa.
+    wp_apply (rcfd_get_spec_aux SpecOwner with "[$]") as ([v |]) ""; last iSteps.
+    iSteps.
+  Qed.
+  #[local] Lemma rcfd_get_spec_closing l γ Ψ `{HΨ : !Fractional Ψ} :
+    {{{
+      inv' l γ Ψ ∗
+      lstate_lb γ LClosingUsers
+    }}}
+      rcfd_get #l
+    {{{
+      RET None : val;
+      True
+    }}}.
+  Proof.
+    iIntros "%Φ (#Hinv & #Hlstate_lb) HΦ".
 
-    iAssert (|==>
-      inv_inner l γ Ψ ∗
-      ( lstate_lb γ LClosingNoUsers
-      ∨ ∃ q,
-        tokens_frag γ q ∗
-        Ψ q
-      )
-    )%I with "[- HΦ]" as ">($ & H)".
-    { destruct lstate1.
-      - iDestruct "Hlstate" as "(:inv_inner_open)".
-        iMod (tokens_update_alloc (q / 2) with "Htokens_auth") as "(Htokens_auth & Htokens_frag)".
-        iDestruct (fractional_half with "HΨ") as "(HΨ1 & HΨ2)"; first done.
-        iSplitR "Htokens_frag HΨ2"; last iSteps.
-        iFrameSteps 2; iPureIntro.
-        + rewrite gmultiset_size_disj_union gmultiset_size_singleton. lia.
-        + rewrite gmultiset_set_fold_disj_union gmultiset_set_fold_singleton Qp.div_2 //.
-      - iDestruct "Hlstate" as "(:inv_inner_closing_users)".
-        iMod (tokens_update_alloc (q / 2) with "Htokens_auth") as "(Htokens_auth & Htokens_frag)".
-        iDestruct (fractional_half with "HΨ") as "(HΨ1 & HΨ2)"; first done.
-        iSplitR "Htokens_frag HΨ2"; last iSteps.
-        iFrameSteps 2; iPureIntro.
-        + rewrite gmultiset_size_disj_union gmultiset_size_singleton. lia.
-        + rewrite gmultiset_size_disj_union. lia.
-        + rewrite gmultiset_set_fold_disj_union gmultiset_set_fold_singleton Qp.div_2 //.
-      - iDestruct "Hlstate" as "(:inv_inner_closing_no_users)".
-        iDestruct (lstate_lb_get with "Hlstate_auth") as "#Hlstate_lb".
-        iFrameSteps 2.
-    }
-
-    iModIntro. wp_pures. clear- HΨ.
-
-    wp_bind (_.{state})%E.
-    iInv "Hinv" as "(:inv_inner =2)".
-    wp_load.
-    destruct (decide (lstate2 = LOpen)) as [-> | Hlstate2].
-
-    - iDestruct "Hlstate" as "(:inv_inner_open)".
-      iDestruct "H" as "[#Hlstate_lb | (%q' & Htokens_frag & HΨ_)]".
-      { iDestruct (lstate_valid_closing_no_users with "Hlstate_auth Hlstate_lb") as %?. done. }
-      iSplitR "Htokens_frag HΨ_ HΦ". { iFrameSteps 2. }
-      iIntros "!> {%}".
-
-      wp_pures.
-      iApply ("HΦ" $! (Some _)). iSteps.
-
-    - iAssert (
-        ∃ fn2,
-        ⌜state2 = Closing fn2⌝
-      )%I as %(fn2 & ->).
-      { destruct lstate2; iDecompose "Hlstate"; iSteps. }
-
-      iSplitR "H HΦ". { iFrameSteps 2. }
-      iModIntro. clear- HΨ.
-
-      wp_smart_apply (rcfd_put_spec with "[$]") as "_".
-      wp_pures.
-      iApply ("HΦ" $! None). iSteps.
+    wp_apply (rcfd_get_spec_aux SpecClosing with "[$]").
+    iSteps.
   Qed.
 
-  Lemma rcfd_use_spec Χ t fd Ψ `{!Fractional Ψ} (closed open : val) :
+  #[local] Lemma rcfd_use_spec_aux spec Χ t owned fd Ψ `{!Fractional Ψ} (closed open : val) :
     {{{
-      rcfd_inv t fd Ψ ∗
+      rcfd_inv t owned fd Ψ ∗
+      specification_pre_1 t spec ∗
+      ( if decide (spec ≠ SpecOwner) then
+          WP closed () {{ Χ false }}
+        else
+          True
+      ) ∗
+      ( if decide (spec ≠ SpecClosing) then
+          ∀ q,
+          Ψ q -∗
+          WP open fd {{ res,
+            Ψ q ∗
+            Χ true res
+          }}
+        else
+          True
+      )
+    }}}
+      rcfd_use t closed open
+    {{{ b res,
+      RET res;
+      Χ b res ∗
+      match spec with
+      | SpecOwner =>
+          ⌜b = true⌝ ∗
+          rcfd_owner t
+      | SpecClosing =>
+          ⌜b = false⌝
+      | SpecNormal =>
+          True
+      end
+    }}}.
+  Proof.
+    iIntros "%Φ ((:inv) & Hspec & Hclosed & Hopen) HΦ".
+    iDestruct (specification_pre_1_2 with "Hmeta Hspec") as "Hspec".
+
+    wp_rec.
+    wp_smart_apply (rcfd_get_spec_aux with "[$]") as ([v |]) "(Hspec & H)".
+
+    - iDestruct "H" as "(%q & -> & Htoken & HΨ)".
+
+      destruct (decide (spec = SpecClosing)) as [-> | Hspec].
+      { iDestruct "Hspec" as %[=]. }
+      iEval (rewrite decide_True //) in "Hopen".
+
+      wp_smart_apply (wp_wand with "(Hopen HΨ)") as "%res (HΨ & HΧ)".
+      wp_smart_apply (rcfd_put_spec with "[Htoken HΨ]") as "_"; first iSteps.
+      wp_pures.
+      destruct spec; try congruence; iSteps.
+
+    - destruct (decide (spec = SpecOwner)) as [-> | Hspec].
+      { iDestruct "Hspec" as "(% & _)". congruence. }
+      iEval (rewrite decide_True //) in "Hclosed".
+
+      wp_smart_apply (wp_wand with "Hclosed") as "%res HΧ".
+      destruct spec; try congruence; iSteps.
+  Qed.
+  Lemma rcfd_use_spec Χ t owned fd Ψ `{!Fractional Ψ} (closed open : val) :
+    {{{
+      rcfd_inv t owned fd Ψ ∗
       WP closed () {{ Χ false }} ∗
       ( ∀ q,
         Ψ q -∗
@@ -618,36 +1036,87 @@ Section rcfd_G.
       Χ b res
     }}}.
   Proof.
-    iIntros "%Φ ((:inv) & Hclosed & Hopen) HΦ".
-    wp_rec.
-    wp_smart_apply (rcfd_get_spec with "Hinv") as ([v |]) ""; last iSteps.
-    iIntros "(%q & -> & Htoken & HΨ)".
-    wp_smart_apply (wp_wand with "(Hopen HΨ)") as "%res (HΨ & HΧ)".
-    wp_smart_apply (rcfd_put_spec with "[Htoken HΨ]"); first iSteps.
+    iIntros "%Φ (#Hinv & Hclosed & Hopen) HΦ".
+
+    wp_apply (rcfd_use_spec_aux SpecNormal with "[$]").
+    iSteps.
+  Qed.
+  Lemma rcfd_use_spec_owner Χ t owned fd Ψ `{!Fractional Ψ} (closed open : val) :
+    {{{
+      rcfd_inv t owned fd Ψ ∗
+      rcfd_owner t ∗
+      ( ∀ q,
+        Ψ q -∗
+        WP open fd {{ res,
+          Ψ q ∗
+          Χ res
+        }}
+      )
+    }}}
+      rcfd_use t closed open
+    {{{ res,
+      RET res;
+      Χ res
+    }}}.
+  Proof.
+    iIntros "%Φ (#Hinv & Howner & Hopen) HΦ".
+
+    wp_apply (rcfd_use_spec_aux SpecOwner (const Χ) with "[$]").
+    iSteps.
+  Qed.
+  Lemma rcfd_use_spec_closing Χ t owned fd Ψ `{!Fractional Ψ} (closed open : val) :
+    {{{
+      rcfd_inv t owned fd Ψ ∗
+      rcfd_closing t ∗
+      WP closed () {{ Χ }}
+    }}}
+      rcfd_use t closed open
+    {{{ res,
+      RET res;
+      Χ res
+    }}}.
+  Proof.
+    iIntros "%Φ (#Hinv & Howner & Hclosed) HΦ".
+
+    wp_apply (rcfd_use_spec_aux SpecClosing (const Χ) with "[$]").
     iSteps.
   Qed.
 
-  #[local] Lemma rcfd_close_spec_aux closing t fd Ψ :
+  #[local] Lemma rcfd_close_spec_aux closing t owned fd Ψ :
     {{{
-      rcfd_inv t fd Ψ ∗
-      if closing then
-        rcfd_closing t
-      else
-        ( Ψ 1%Qp -∗
+      rcfd_inv t owned fd Ψ ∗
+      ( if owned then
+          rcfd_owner t
+        else
+          True
+      ) ∗
+      ( if closing then
+          rcfd_closing t
+        else
+          Ψ 1%Qp -∗
             ∃ chars,
             unix_fd_model fd (DfracOwn 1) chars
-        )
+      )
     }}}
       rcfd_close t
     {{{ b,
       RET #b;
-      if closing then
-        ⌜b = false⌝
-      else
-        rcfd_closing t
+      rcfd_closing t ∗
+      ( if owned then
+          ⌜b = true⌝
+        else
+          True
+      ) ∗
+      ( if closing then
+          ⌜b = false⌝
+        else
+          True
+      )
     }}}.
   Proof.
-    iIntros "%Φ ((:inv) & Hclosing) HΦ".
+    iIntros "%Φ ((:inv) & Howner & Hclosing) HΦ".
+    iDestruct (rcfd_owner_elim' with "Hmeta Howner") as "Howner".
+    iDestruct (rcfd_closing_elim' with "Hmeta Hclosing") as "Hclosing".
 
     wp_rec. wp_pures.
 
@@ -656,14 +1125,12 @@ Section rcfd_G.
     wp_load.
     destruct (decide (lstate1 = LOpen)) as [-> | Hlstate1].
 
-    - iDestruct "Hlstate" as "(:inv_inner_open =1)".
-      destruct closing.
-      { iDestruct "Hclosing" as "(:closing)". injection Heq as <-.
-        iDestruct (meta_agree with "Hmeta Hmeta_") as %<-. iClear "Hmeta_".
-        iDestruct (lstate_valid_closing_users with "Hlstate_auth Hlstate_lb") as %[[=] | [=]].
-      }
+    - iDestruct "Hlstate" as "(:inv_lstate_open =1)".
 
-      iSplitR "Hclosing HΦ". { iFrameSteps 2. }
+      destruct closing.
+      { iDestruct (lstate_valid_closing_users with "Hlstate_auth Hclosing") as %?. congruence. }
+
+      iSplitR "Howner Hclosing HΦ". { iFrameSteps 2. }
       iIntros "!> {%}".
 
       wp_pures.
@@ -672,35 +1139,26 @@ Section rcfd_G.
       iInv "Hinv" as "(:inv_inner =2)".
       wp_cas as Hcas.
 
-      + iAssert (
-          ∃ fn2,
-          ⌜state2 = Closing fn2⌝ ∗
-          lstate_lb γ LClosingUsers
-        )%I as "(%fn2 & -> & #Hlstate_lb)".
-        { destruct lstate2; iDecompose "Hlstate".
-          - zoo_simpl. naive_solver.
-          - iDestruct (lstate_lb_get with "Hlstate_auth") as "$".
-            iSteps.
-          - iDestruct (lstate_lb_get with "Hlstate_auth") as "Hlstate_lb".
-            iDestruct (lstate_lb_mono with "Hlstate_lb") as "$"; first done.
-            iSteps.
-        }
+      + iDestruct (inv_lstate_Closing with "Hlstate Hlstate_auth") as "(%fn2 & -> & %Hlstate2 & #Hlstate_lb)".
+        { intros ->. zoo_simpl. naive_solver. }
+
+        destruct γ.(metadata_owned).
+        { iDestruct (owner_lstate_auth with "Howner Hlstate_auth") as %->. congruence. }
 
         iSplitR "HΦ". { iFrameSteps 2. }
         iSteps.
 
       + destruct state2; last zoo_simpl.
-        destruct (decide (lstate2 = LOpen)) as [-> | Hlstate2]; last first.
-        { destruct lstate2; iDecompose "Hlstate"; iSteps. }
-        iDestruct "Hlstate" as "(:inv_inner_open =2 eq)".
-        iMod (lstate_update LClosingUsers with "Hlstate_auth") as "Hlstate_auth"; first done.
-        iDestruct (lstate_lb_get with "Hlstate_auth") as "#Hlstate_lb".
+        iDestruct (inv_lstate_Open with "Hlstate") as %->.
+        iDestruct "Hlstate" as "(:inv_lstate_open =2 eq)".
 
+        iMod (lstate_update_close_users with "Hlstate_auth Howner") as "Hlstate_auth".
+        iDestruct (lstate_lb_get with "Hlstate_auth") as "#Hlstate_lb".
         iSplitR "HΦ".
         { destruct (decide (size qs2 = 0)) as [Hqs_size | Hqs_size].
           - apply gmultiset_size_empty_iff in Hqs_size as ->.
             rewrite gmultiset_set_fold_empty in Hqs2. rewrite {}Hqs2.
-            iMod (lstate_update LClosingNoUsers with "Hlstate_auth") as "Hlstate_auth"; first done.
+            iMod (lstate_update_close_no_users with "Hlstate_auth") as "Hlstate_auth".
             iDestruct ("Hclosing" with "HΨ") as "(%chars & Hfd)".
             iExists (Closing _). iFrameSteps.
           - iExists (Closing _). iFrame. iStep 8 as "HΨ".
@@ -710,20 +1168,12 @@ Section rcfd_G.
         iIntros "!> {%}".
 
         wp_smart_apply (rcfd_finish_spec with "[$]").
-        iSteps.
+        destruct γ.(metadata_owned); iSteps.
 
-    - iAssert (
-        ∃ fn1,
-        ⌜state1 = Closing fn1⌝ ∗
-        lstate_lb γ LClosingUsers
-      )%I as "(%fn1 & -> & #Hlstate_lb)".
-      { destruct lstate1; iDecompose "Hlstate".
-        - iDestruct (lstate_lb_get with "Hlstate_auth") as "$".
-          iSteps.
-        - iDestruct (lstate_lb_get with "Hlstate_auth") as "Hlstate_lb".
-          iDestruct (lstate_lb_mono with "Hlstate_lb") as "$"; first done.
-          iSteps.
-      }
+    - iDestruct (inv_lstate_LClosing with "Hlstate Hlstate_auth") as "(%fn1 & -> & #Hlstate_lb)"; first done.
+
+      destruct γ.(metadata_owned).
+      { iDestruct (owner_lstate_auth with "Howner Hlstate_auth") as %->. congruence. }
 
       iSplitR "HΦ". { iFrameSteps 2. }
       iIntros "!> {%}".
@@ -731,9 +1181,14 @@ Section rcfd_G.
       wp_pures.
       destruct closing; iSteps.
   Qed.
-  Lemma rcfd_close_spec t fd Ψ :
+  Lemma rcfd_close_spec t owned fd Ψ :
     {{{
-      rcfd_inv t fd Ψ ∗
+      rcfd_inv t owned fd Ψ ∗
+      ( if owned then
+          rcfd_owner t
+        else
+          True
+      ) ∗
       ( Ψ 1%Qp -∗
           ∃ chars,
           unix_fd_model fd (DfracOwn 1) chars
@@ -742,15 +1197,21 @@ Section rcfd_G.
       rcfd_close t
     {{{ b,
       RET #b;
-      rcfd_closing t
+      rcfd_closing t ∗
+      if owned then
+        ⌜b = true⌝
+      else
+        True
     }}}.
   Proof.
-    iIntros "%Φ (#Hinv & H) HΦ".
-    wp_apply (rcfd_close_spec_aux false with "[$] HΦ").
+    iIntros "%Φ (#Hinv & Howner & H) HΦ".
+
+    wp_apply (rcfd_close_spec_aux false with "[$]").
+    iSteps.
   Qed.
   Lemma rcfd_close_spec_closing t fd Ψ :
     {{{
-      rcfd_inv t fd Ψ ∗
+      rcfd_inv t false fd Ψ ∗
       rcfd_closing t
     }}}
       rcfd_close t
@@ -760,35 +1221,51 @@ Section rcfd_G.
     }}}.
   Proof.
     iIntros "%Φ (#Hinv & #Hclosing) HΦ".
+
     wp_apply (rcfd_close_spec_aux true with "[$]").
     iSteps.
   Qed.
 
-  #[local] Lemma rcfd_remove_spec_aux closing t fd Ψ :
+  #[local] Lemma rcfd_remove_spec_aux closing t owned fd Ψ :
     {{{
-      rcfd_inv t fd Ψ ∗
-      if closing then
-        rcfd_closing t
-      else
-        True
+      rcfd_inv t owned fd Ψ ∗
+      ( if owned then
+          rcfd_owner t
+        else
+          True
+      ) ∗
+      ( if closing then
+          rcfd_closing t
+        else
+          True
+      )
     }}}
       rcfd_remove t
     {{{ o,
       RET (o : val);
-      if closing then
-        ⌜o = None⌝
-      else
-        rcfd_closing t ∗
-        match o with
-        | None =>
-            True
-        | Some fd_ =>
-            ⌜fd_ = fd⌝ ∗
-            Ψ 1%Qp
-        end
+      rcfd_closing t ∗
+      ( if owned then
+          ⌜o = Some fd⌝ ∗
+          Ψ 1%Qp
+        else
+          match o with
+          | None =>
+              True
+          | Some fd_ =>
+              ⌜fd_ = fd⌝ ∗
+              Ψ 1%Qp
+          end
+      ) ∗
+      ( if closing then
+          ⌜o = None⌝
+        else
+          True
+      )
     }}}.
   Proof.
-    iIntros "%Φ ((:inv) & Hclosing) HΦ".
+    iIntros "%Φ ((:inv) & Howner & Hclosing) HΦ".
+    iDestruct (rcfd_owner_elim' with "Hmeta Howner") as "Howner".
+    iDestruct (rcfd_closing_elim' with "Hmeta Hclosing") as "Hclosing".
 
     wp_rec. wp_pures.
 
@@ -797,14 +1274,12 @@ Section rcfd_G.
     wp_load.
     destruct (decide (lstate1 = LOpen)) as [-> | Hlstate1].
 
-    - iDestruct "Hlstate" as "(:inv_inner_open =1)".
-      destruct closing; last iClear "Hclosing".
-      { iDestruct "Hclosing" as "(:closing)". injection Heq as <-.
-        iDestruct (meta_agree with "Hmeta Hmeta_") as %<-. iClear "Hmeta_".
-        iDestruct (lstate_valid_closing_users with "Hlstate_auth Hlstate_lb") as %[[=] | [=]].
-      }
+    - iDestruct "Hlstate" as "(:inv_lstate_open =1)".
 
-      iSplitR "HΦ". { iFrameSteps 2. }
+      destruct closing.
+      { iDestruct (lstate_valid_closing_users with "Hlstate_auth Hclosing") as %?. congruence. }
+
+      iSplitR "Howner HΦ". { iFrameSteps 2. }
       iIntros "!> {%}".
 
       wp_smart_apply (spsc_waiter_create_spec (Ψ 1%Qp) with "[//]") as "%waiter (#Hwaiter_inv & Hwaiter_producer & Hwaiter_consumer)".
@@ -814,37 +1289,30 @@ Section rcfd_G.
       iInv "Hinv" as "(:inv_inner =2)".
       wp_cas as Hcas.
 
-      + iAssert (
-          ∃ fn2,
-          ⌜state2 = Closing fn2⌝ ∗
-          lstate_lb γ LClosingUsers
-        )%I as "(%fn2 & -> & #Hlstate_lb)".
-        { destruct lstate2; iDecompose "Hlstate".
-          - zoo_simpl. naive_solver.
-          - iDestruct (lstate_lb_get with "Hlstate_auth") as "$".
-            iSteps.
-          - iDestruct (lstate_lb_get with "Hlstate_auth") as "Hlstate_lb".
-            iDestruct (lstate_lb_mono with "Hlstate_lb") as "$"; first done.
-            iSteps.
-        }
+      + iDestruct (inv_lstate_Closing with "Hlstate Hlstate_auth") as "(%fn2 & -> & %Hlstate2 & #Hlstate_lb)".
+        { intros ->. zoo_simpl. naive_solver. }
+
+        destruct γ.(metadata_owned).
+        { iDestruct (owner_lstate_auth with "Howner Hlstate_auth") as %->. congruence. }
 
         iSplitR "HΦ". { iFrameSteps 2. }
         iIntros "!> {%}".
 
         wp_pures.
-        iApply ("HΦ" $! None). iSteps.
+        iApply ("HΦ" $! None).
+        iSteps.
 
       + destruct state2; last zoo_simpl.
-        destruct (decide (lstate2 = LOpen)) as [-> | Hlstate2]; last first.
-        { destruct lstate2; iDecompose "Hlstate"; iSteps. }
-        iDestruct "Hlstate" as "(:inv_inner_open =2 eq)".
-        iMod (lstate_update LClosingUsers with "Hlstate_auth") as "Hlstate_auth"; first done.
+        iDestruct (inv_lstate_Open with "Hlstate") as %->.
+        iDestruct "Hlstate" as "(:inv_lstate_open =2 eq)".
+
+        iMod (lstate_update_close_users with "Hlstate_auth Howner") as "Hlstate_auth".
         iDestruct (lstate_lb_get with "Hlstate_auth") as "#Hlstate_lb".
         iSplitR "Hwaiter_consumer HΦ".
         { destruct (decide (size qs2 = 0)) as [Hqs_size | Hqs_size].
           - apply gmultiset_size_empty_iff in Hqs_size as ->.
             rewrite gmultiset_set_fold_empty in Hqs2. rewrite {}Hqs2.
-            iMod (lstate_update LClosingNoUsers with "Hlstate_auth") as "Hlstate_auth"; first done.
+            iMod (lstate_update_close_no_users with "Hlstate_auth") as "Hlstate_auth".
             iExists (Closing _). iFrameStep 8.
             wp_apply (spsc_waiter_notify_spec with "[$Hwaiter_inv $Hwaiter_producer $HΨ]").
             iSteps.
@@ -856,50 +1324,54 @@ Section rcfd_G.
 
         wp_smart_apply (spsc_waiter_wait_spec with "[$Hwaiter_inv $Hwaiter_consumer]") as "HΨ".
         wp_pures.
-        iApply ("HΦ" $! (Some _)). iSteps.
+        iApply ("HΦ" $! (Some _)).
+        destruct γ.(metadata_owned); iSteps.
 
-    - iAssert (
-        ∃ fn1,
-        ⌜state1 = Closing fn1⌝ ∗
-        lstate_lb γ LClosingUsers
-      )%I as "(%fn1 & -> & #Hlstate_lb)".
-      { destruct lstate1; iDecompose "Hlstate".
-        - iDestruct (lstate_lb_get with "Hlstate_auth") as "$".
-          iSteps.
-        - iDestruct (lstate_lb_get with "Hlstate_auth") as "Hlstate_lb".
-          iDestruct (lstate_lb_mono with "Hlstate_lb") as "$"; first done.
-          iSteps.
-      }
+    - iDestruct (inv_lstate_LClosing with "Hlstate Hlstate_auth") as "(%fn1 & -> & #Hlstate_lb)"; first done.
+
+      destruct γ.(metadata_owned).
+      { iDestruct (owner_lstate_auth with "Howner Hlstate_auth") as %->. congruence. }
 
       iSplitR "HΦ". { iFrameSteps 2. }
       iIntros "!> {%}".
 
       wp_pures.
-      iApply ("HΦ" $! None). destruct closing; iSteps.
+      iApply ("HΦ" $! None).
+      destruct closing; iSteps.
   Qed.
-  Lemma rcfd_remove_spec t fd Ψ :
+  Lemma rcfd_remove_spec t owned fd Ψ :
     {{{
-      rcfd_inv t fd Ψ
+      rcfd_inv t owned fd Ψ ∗
+      if owned then
+        rcfd_owner t
+      else
+        True
     }}}
       rcfd_remove t
     {{{ o,
       RET (o : val);
       rcfd_closing t ∗
-      match o with
-      | None =>
-          True
-      | Some fd_ =>
-          ⌜fd_ = fd⌝ ∗
-          Ψ 1%Qp
-      end
+      if owned then
+        ⌜o = Some fd⌝ ∗
+        Ψ 1%Qp
+      else
+        match o with
+        | None =>
+            True
+        | Some fd_ =>
+            ⌜fd_ = fd⌝ ∗
+            Ψ 1%Qp
+        end
     }}}.
   Proof.
-    iIntros "%Φ #Hinv HΦ".
-    wp_apply (rcfd_remove_spec_aux false with "[$Hinv] HΦ").
+    iIntros "%Φ (#Hinv & Howner) HΦ".
+
+    wp_apply (rcfd_remove_spec_aux false with "[$]").
+    iSteps.
   Qed.
-  Lemma rcfd_remove_spec_closing closing t fd Ψ :
+  Lemma rcfd_remove_spec_closing t fd Ψ :
     {{{
-      rcfd_inv t fd Ψ ∗
+      rcfd_inv t false fd Ψ ∗
       rcfd_closing t
     }}}
       rcfd_remove t
@@ -909,70 +1381,68 @@ Section rcfd_G.
     }}}.
   Proof.
     iIntros "%Φ (#Hinv & #Hclosing) HΦ".
-    wp_apply (rcfd_remove_spec_aux true with "[$Hinv $Hclosing]").
+
+    wp_apply (rcfd_remove_spec_aux true with "[$]").
     iSteps.
   Qed.
 
-  #[local] Lemma rcfd_is_open_spec_aux closing t fd Ψ :
+  #[local] Lemma rcfd_is_open_spec_aux spec t owned fd Ψ :
     {{{
-      rcfd_inv t fd Ψ ∗
-      if closing then
-        rcfd_closing t
-      else
-        True
+      rcfd_inv t owned fd Ψ ∗
+      specification_pre_1 t spec
     }}}
       rcfd_is_open t
     {{{ b,
       RET #b;
-      if closing then
-        ⌜b = false⌝
-      else if b then
-        True
-      else
-        rcfd_closing t
+      match spec with
+      | SpecOwner =>
+          ⌜b = true⌝ ∗
+          rcfd_owner t
+      | SpecClosing =>
+          ⌜b = false⌝
+      | SpecNormal =>
+          if b then
+            True
+          else
+            rcfd_closing t
+      end
     }}}.
   Proof.
-    iIntros "%Φ ((:inv) & Hclosing) HΦ".
+    iIntros "%Φ ((:inv) & Hspec) HΦ".
+    iDestruct (specification_pre_1_2 with "Hmeta Hspec") as "Hspec".
 
     wp_rec. wp_pures.
 
     wp_bind (_.{state})%E.
     iInv "Hinv" as "(:inv_inner)".
     wp_load.
-    destruct closing.
+    destruct state as [| fn].
 
-    - iDestruct "Hclosing" as "(:closing)". injection Heq as <-.
-      iDestruct (meta_agree with "Hmeta Hmeta_") as %<-. iClear "Hmeta_".
+    - iDestruct (inv_lstate_Open with "Hlstate") as %->.
 
-      iAssert (
-        ∃ fn,
-        ⌜state = Closing fn⌝
-      )%I as "(%fn & ->)".
-      { iDestruct (lstate_valid_closing_users with "Hlstate_auth Hlstate_lb") as %[-> | ->].
-        all: iDecompose "Hlstate"; iSteps.
-      }
+      destruct (decide (spec = SpecClosing)) as [-> | Hspec].
+      { iDestruct (lstate_valid_closing_users with "Hlstate_auth Hspec") as %?. congruence. }
+
+      iSplitR "Hspec HΦ". { iFrameSteps 2. }
+      iModIntro. clear- Hspec.
+
+      wp_pures.
+      destruct spec; try congruence; iSteps.
+
+    - iDestruct (inv_lstate_Closing with "Hlstate Hlstate_auth") as "#(%fn_ & _ & %Hlstate & #Hlstate_lb)"; first done.
+
+      destruct (decide (spec = SpecOwner)) as [-> | Hspec].
+      { iDestruct (owner_lstate_auth with "Hspec Hlstate_auth") as %->. congruence. }
 
       iSplitR "HΦ". { iFrameSteps 2. }
-      iSteps.
+      iModIntro. clear- Hspec.
 
-    - destruct state.
-
-      + iSplitR "HΦ". { iFrameSteps 2. }
-        iSteps.
-
-      + iAssert (lstate_lb γ LClosingUsers) as "#Hlstate_lb".
-        { destruct lstate; iDecompose "Hlstate".
-          - iApply (lstate_lb_get with "Hlstate_auth").
-          - iDestruct (lstate_lb_get with "Hlstate_auth") as "Hlstate_lb".
-            iApply (lstate_lb_mono with "Hlstate_lb"); first done.
-        }
-
-        iSplitR "HΦ". { iFrameSteps 2. }
-        iSteps.
+      wp_pures.
+      destruct spec; try congruence; iSteps.
   Qed.
-  Lemma rcfd_is_open_spec t fd Ψ :
+  Lemma rcfd_is_open_spec t owned fd Ψ :
     {{{
-      rcfd_inv t fd Ψ
+      rcfd_inv t owned fd Ψ
     }}}
       rcfd_is_open t
     {{{ b,
@@ -984,11 +1454,29 @@ Section rcfd_G.
     }}}.
   Proof.
     iIntros "%Φ #Hinv HΦ".
-    wp_apply (rcfd_is_open_spec_aux false with "[$Hinv] HΦ").
+
+    wp_apply (rcfd_is_open_spec_aux SpecNormal with "[$]").
+    iSteps.
   Qed.
-  Lemma rcfd_is_open_spec_closing t fd Ψ :
+  Lemma rcfd_is_open_spec_owner t owned fd Ψ :
     {{{
-      rcfd_inv t fd Ψ ∗
+      rcfd_inv t owned fd Ψ ∗
+      rcfd_owner t
+    }}}
+      rcfd_is_open t
+    {{{
+      RET #true;
+      rcfd_owner t
+    }}}.
+  Proof.
+    iIntros "%Φ (#Hinv & Howner) HΦ".
+
+    wp_apply (rcfd_is_open_spec_aux SpecOwner with "[$]").
+    iSteps.
+  Qed.
+  Lemma rcfd_is_open_spec_closing t owned fd Ψ :
+    {{{
+      rcfd_inv t false fd Ψ ∗
       rcfd_closing t
     }}}
       rcfd_is_open t
@@ -998,82 +1486,72 @@ Section rcfd_G.
     }}}.
   Proof.
     iIntros "%Φ (#Hinv & #Hclosing) HΦ".
-    wp_apply (rcfd_is_open_spec_aux true with "[$Hinv $Hclosing]").
+
+    wp_apply (rcfd_is_open_spec_aux SpecClosing with "[$]").
     iSteps.
   Qed.
 
-  #[local] Lemma rcfd_peek_spec_aux closing t fd Ψ :
+  #[local] Lemma rcfd_peek_spec_aux spec t owned fd Ψ :
     {{{
-      rcfd_inv t fd Ψ ∗
-      if closing then
-        rcfd_closing t
-      else
-        True
+      rcfd_inv t owned fd Ψ ∗
+      specification_pre_1 t spec
     }}}
       rcfd_peek t
     {{{ o,
       RET (o : val);
-      if closing then
-        ⌜o = None⌝
-      else
-        match o with
-        | None =>
-            rcfd_closing t
-        | Some fd_ =>
-            ⌜fd_ = fd⌝
-        end
+      match spec with
+      | SpecOwner =>
+          ⌜o = Some fd⌝ ∗
+          rcfd_owner t
+      | SpecClosing =>
+          ⌜o = None⌝
+      | SpecNormal =>
+          match o with
+          | None =>
+              rcfd_closing t
+          | Some fd_ =>
+              ⌜fd_ = fd⌝
+          end
+      end
     }}}.
   Proof.
-    iIntros "%Φ ((:inv) & Hclosing) HΦ".
+    iIntros "%Φ ((:inv) & Hspec) HΦ".
+    iDestruct (specification_pre_1_2 with "Hmeta Hspec") as "Hspec".
 
     wp_rec. wp_pures.
 
     wp_bind (_.{state})%E.
     iInv "Hinv" as "(:inv_inner)".
     wp_load.
-    destruct closing.
+    destruct state as [| fn].
 
-    - iDestruct "Hclosing" as "(:closing)". injection Heq as <-.
-      iDestruct (meta_agree with "Hmeta Hmeta_") as %<-. iClear "Hmeta_".
+    - iDestruct (inv_lstate_Open with "Hlstate") as %->.
 
-      iAssert (
-        ∃ fn,
-        ⌜state = Closing fn⌝
-      )%I as "(%fn & ->)".
-      { iDestruct (lstate_valid_closing_users with "Hlstate_auth Hlstate_lb") as %[-> | ->].
-        all: iDecompose "Hlstate"; iSteps.
-      }
+      destruct (decide (spec = SpecClosing)) as [-> | Hspec].
+      { iDestruct (lstate_valid_closing_users with "Hlstate_auth Hspec") as %?. congruence. }
 
-      iSplitR "HΦ". { iFrameSteps 2. }
-      iIntros "!> {%}".
+      iSplitR "Hspec HΦ". { iFrameSteps 2. }
+      iModIntro. clear- Hspec.
 
       wp_pures.
-      iApply ("HΦ" $! None). iSteps.
+      iApply ("HΦ" $! (Some _)).
+      destruct spec; try congruence; iSteps.
 
-    - destruct state.
+    - iDestruct (inv_lstate_Closing with "Hlstate Hlstate_auth") as "#(%fn_ & _ & %Hlstate & #Hlstate_lb)"; first done.
 
-      + iSplitR "HΦ". { iFrameSteps 2. }
-        iIntros "!> {%}".
+      destruct (decide (spec = SpecOwner)) as [-> | Hspec].
+      { iDestruct (owner_lstate_auth with "Hspec Hlstate_auth") as %->. congruence. }
 
-        wp_pures.
-        iApply ("HΦ" $! (Some _)). iSteps.
+      iSplitR "HΦ". { iFrameSteps 2. }
+      iModIntro. clear- Hspec.
 
-      + iAssert (lstate_lb γ LClosingUsers) as "#Hlstate_lb".
-        { destruct lstate; iDecompose "Hlstate".
-          - iApply (lstate_lb_get with "Hlstate_auth").
-          - iDestruct (lstate_lb_get with "Hlstate_auth") as "Hlstate_lb".
-            iApply (lstate_lb_mono with "Hlstate_lb"); first done.
-        }
-
-        iSplitR "HΦ". { iFrameSteps 2. }
-        iIntros "!> {%}".
-
-        wp_pures.
-        iApply ("HΦ" $! None). iSteps.
+      wp_pures.
+      iApply ("HΦ" $! None).
+      destruct spec; try congruence; iSteps.
   Qed.
-  Lemma rcfd_peek_spec t fd Ψ :
+  Lemma rcfd_peek_spec t owned fd Ψ :
     {{{
-      rcfd_inv t fd Ψ
+      rcfd_inv t owned fd Ψ
     }}}
       rcfd_peek t
     {{{ o,
@@ -1087,11 +1565,29 @@ Section rcfd_G.
     }}}.
   Proof.
     iIntros "%Φ #Hinv HΦ".
-    wp_apply (rcfd_peek_spec_aux false with "[$Hinv] HΦ").
+
+    wp_apply (rcfd_peek_spec_aux SpecNormal with "[$]").
+    iSteps.
   Qed.
-  Lemma rcfd_peek_spec_closing t fd Ψ :
+  Lemma rcfd_peek_spec_owner t owned fd Ψ :
     {{{
-      rcfd_inv t fd Ψ ∗
+      rcfd_inv t owned fd Ψ ∗
+      rcfd_owner t
+    }}}
+      rcfd_peek t
+    {{{
+      RET Some fd : val;
+      rcfd_owner t
+    }}}.
+  Proof.
+    iIntros "%Φ (#Hinv & Howner) HΦ".
+
+    wp_apply (rcfd_peek_spec_aux SpecOwner with "[$]").
+    iSteps.
+  Qed.
+  Lemma rcfd_peek_spec_closing t owned fd Ψ :
+    {{{
+      rcfd_inv t owned fd Ψ ∗
       rcfd_closing t
     }}}
       rcfd_peek t
@@ -1101,7 +1597,8 @@ Section rcfd_G.
     }}}.
   Proof.
     iIntros "%Φ (#Hinv & #Hclosing) HΦ".
-    wp_apply (rcfd_peek_spec_aux true with "[$Hinv $Hclosing]").
+
+    wp_apply (rcfd_peek_spec_aux SpecClosing with "[$]").
     iSteps.
   Qed.
 End rcfd_G.
@@ -1110,4 +1607,5 @@ From zoo_eio Require
   rcfd__opaque.
 
 #[global] Opaque rcfd_inv.
+#[global] Opaque rcfd_owner.
 #[global] Opaque rcfd_closing.
